define semantic typing

Semantic/Stlc/Soundness.lean
@@ -1,1 +1,108 @@
 import Semantic.Stlc.TypeSystem
+import Semantic.Stlc.Interpreter
+import Mathlib.Tactic
+
+structure Config (n : Nat) where
+  s : Store n
+  e : Exp n
+
+mutual
+
+def Ty.val_denot : Ty -> ∀ {n}, Config n -> Prop
+| .bool => fun config =>
+  config.e.is_bool_val
+| .nat => fun config =>
+  config.e.is_num_val
+| .arrow T U => fun config =>
+  ∀ arg_v,
+    Ty.val_denot T ⟨config.s, arg_v⟩ ->
+    Ty.exp_denot U ⟨config.s, .app config.e arg_v⟩
+
+def Ty.exp_denot : Ty -> ∀ {n}, Config n -> Prop
+| T => fun config =>
+  ∃ fuel v,
+    eval config.s config.e fuel = .ok v
+    ∧ Ty.val_denot T ⟨config.s, v⟩
+
+end
+
+def TypedStore : Store n -> Ctx n -> Prop
+| .empty, .empty => True
+| .val s v, .var Γ T =>
+  TypedStore s Γ ∧ Ty.val_denot T ⟨s, v⟩
+
+def SemanticTyping (Γ : Ctx n) (e : Exp n) (T : Ty) : Prop :=
+  ∀ s,
+    TypedStore s Γ ->
+    Ty.exp_denot T ⟨s, e⟩
+
+notation:65 Γ " ⊨ " e " : " T => SemanticTyping Γ e T
+
+theorem typed_store_lookup
+  (hts : TypedStore s Γ)
+  (hb : Ctx.Lookup Γ x T) :
+  Ty.val_denot T ⟨s, s.lookup x⟩ := by
+  induction hb
+  case here =>
+    cases s; rename_i s0 v0
+    simp [TypedStore] at hts
+    simp [Store.lookup]
+    sorry
+  case there ih => sorry
+
+theorem sem_typ_var
+  (hb : Ctx.Lookup Γ x T) :
+  (Γ ⊨ (.var x) : T) := by
+  intro s hts
+  simp [Ty.exp_denot]
+  use 1, s.lookup x
+  split_ands
+  { rfl }
+  { sorry }
+
+theorem sem_typ_nsucc
+  (ht : Γ ⊨ e : Ty.nat) :
+  (Γ ⊨ .nsucc e : Ty.nat) := by
+  intro s hts
+  specialize ht s hts
+  simp [Ty.exp_denot] at *
+  have ⟨fuel0, v0, hev0, hv0⟩ := ht
+  simp [Ty.val_denot] at hv0
+  use fuel0+1, .nsucc v0
+  split_ands
+  { grind [eval] }
+  { simp [Ty.val_denot]
+    grind [Exp.is_num_val] }
+
+theorem soundness
+  (ht : Γ ⊢ e : T) :
+  (Γ ⊨ e : T) := by
+  induction ht
+  case var => sorry
+  case abs => sorry
+  case app => sorry
+  case btrue =>
+    intro s hts
+    simp [Ty.exp_denot]
+    use 1, .btrue
+    split_ands
+    { rfl }
+    { simp [Ty.val_denot]; rfl }
+  case bfalse =>
+    intro s hts
+    simp [Ty.exp_denot]
+    use 1, .bfalse
+    split_ands
+    { rfl }
+    { simp [Ty.val_denot]; rfl }
+  case nzero =>
+    intro s hts
+    simp [Ty.exp_denot]
+    use 1, .nzero
+    split_ands
+    { rfl }
+    { simp [Ty.val_denot]; rfl }
+  case nsucc ih => apply sem_typ_nsucc ih
+  case pred => sorry
+  case iszero => sorry
+  case cond => sorry
